\documentclass[12pt]{article}
\pagestyle{empty}
\usepackage{amsmath, amssymb, amsthm}
\usepackage{latexsym, epsfig, ulem, cancel, multicol, hyperref}
\usepackage{graphicx, tikz, subfigure,pgfplots}
\usepackage[margin=1in]{geometry}
\setlength{\parindent}{0pt}
\usepackage{multirow}
\usepackage{mathtools}


\newcommand{\R}{\mathbb{R}}
\newcommand{\dydx}{\frac{dy}{dx}}
\usepackage{verbatim}
\usepackage{tikz}
\usepackage{pgfplots}

\newcommand{\wsnumber}{1}
\newcommand{\wstopic}{Vectors}
\pgfplotsset{
    every linear axis/.append style={
       axis x line=center,
       axis y line=center,
       xlabel={$x$},
       ylabel={$y$}
    },
    every axis plot/.append style={thick,mark=none}
}
\tikzset{
    point/.style={circle,draw,fill,minimum width=0.3ex,inner sep=0pt,outer sep=0pt},
    every label/.append style={black}
}


\usepackage[margin=1in]{geometry}
\usepackage{amsmath, amssymb, amsthm, graphicx, hyperref}
\usepackage{enumerate}
\usepackage{fancyhdr}
\usepackage{multirow, multicol}
\usepackage{tikz}
\pagestyle{fancy}
\fancyhead[RO]{Summer 6W2 2024}
\fancyhead[LO]{MA-UY 2314 Discrete Mathematics}
\usepackage{comment}
\newif\ifshow
\showfalse

\ifshow
  \newenvironment{solution}{\textbf{Solution.}}{}
\else
  \excludecomment{solution}
\fi

\renewcommand{\thefootnote}{\fnsymbol{footnote}}
\usepackage{comment}

\newcommand{\T}[0]{\top}
\newcommand{\F}[0]{\bot}

\newtheorem*{remark}{Remark}


\begin{document}

\begin{center}
\ifshow
  \textbf{\Large Formula Sheet 2.1.1.}\\
\else
  \textbf{\Large Theorem 2.1.1}\\
\fi
Reference\\
Discrete Mathematics with Applications 5th. ED. \\
Susanna S. Epp\\
\end{center}

\hrule

\vspace{0.2cm}

\hrule

\vspace{0.5cm}



\begin{enumerate}

    \item[0.] Theorem *\\
    Let $p$ and $q$ be statement variables, then
        \[
        p \rightarrow q \equiv \neg p \vee q
        \]

    \item Commutativity
        \[
        p \vee q \equiv q \vee p
        \]
        \[
        p \wedge q \equiv q \wedge p
        \]
    \item Associativity
        \[
        (p \vee q) \vee r \equiv p \vee (q\vee r)
        \]
        \[
        (p \wedge q) \wedge r \equiv p \wedge (q\wedge r)
        \]
    \item Distributivity
        \[
        p \vee (q \wedge r) \equiv (p \vee q) \wedge (p \vee r)
        \]
        \[
        p \wedge (q \vee r) \equiv (p \wedge q) \vee (p \wedge r)
        \]
    \item Identity Laws
        \[
        p \wedge \T \equiv p
        \]
        \[
        p \vee \F \equiv p
        \]
    \item Negation Laws
        \[
        p \vee \neg p \equiv \T
        \]
        \[
        p \wedge \neg p \equiv \F
        \]
    \item Double Negative Law
        \[
        \neg (\neg p) \equiv p
        \]
    \item Idempotence
        \[
        p \vee p \equiv p
        \]
        \[
        p \wedge p \equiv p
        \]
    \item Universal Bound
        \[
        p \vee \T \equiv \T
        \]
        \[
        p \wedge \F \equiv \F
        \]
    \item DeMorgan's Laws
        \[
        \neg (p \vee q) \equiv \neg p \wedge \neg q
        \]
        \[
        \neg (p \wedge q) \equiv \neg p \vee \neg q
        \]
    \item Absorption Laws
        \[
        p \vee (p \wedge q) \equiv p
        \]
        \[
        p \wedge (p \vee q) \equiv p
        \]
    \item Tautology and Contradiction Negation
        \[
        \neg \T \equiv \F
        \]
        \[
        \neg \F \equiv \T
        \]

\end{enumerate}

\newpage

\begin{enumerate}
    \item[0.] Modus Ponens
        \[
        \begin{array}{c}
        p \rightarrow q \\
        p \\
        \therefore q
        \end{array}
        \]
    \item Modus Tollens
        \[
        \begin{array}{c}
        p \rightarrow q \\
        \neg q \\
        \therefore \neg p
        \end{array}
        \]
    \item Generalization
        \[
        \begin{array}{ll}
        a. & p \\
        & \therefore p \vee q
        \end{array}
        \]
        \[
        \begin{array}{ll}
        b. & q \\
        & \therefore p \vee q
        \end{array}
        \]
    \item Specialization
        \[
        \begin{array}{ll}
        a. & p \wedge q \\
        & \therefore p
        \end{array}
        \]
        \[
        \begin{array}{ll}
        b. & p \wedge q \\
        & \therefore q
        \end{array}
        \]
    \item Conjunction
        \[
        \begin{array}{c}
        p \\
        q \\
        \therefore p \wedge q
        \end{array}
        \]
    \item Elimination
        \[
        \begin{array}{ll}
        a. & p \vee q \\
        & \neg q \\
        & \therefore p
        \end{array}
        \]
        \[
        \begin{array}{ll}
        b. & p \vee q \\
        & \neg p \\
        & \therefore q
        \end{array}
        \]
    \item Transitivity
        \[
        \begin{array}{c}
        p \rightarrow q \\
        q \rightarrow r \\
        \therefore p \rightarrow r
        \end{array}
        \]
    \item Proof by Division into Cases
        \[
        \begin{array}{c}
        p \vee q \\
        p \rightarrow r \\
        q \rightarrow r \\
        \therefore r
        \end{array}
        \]
    \item Contradiction Rule
        \[
        \begin{array}{c}
        \neg p \rightarrow c \\
        \therefore p
        \end{array}
        \]
\end{enumerate}
\newpage
\section{Theorem 6.2.2}
\begin{enumerate}

    \item \textbf{Commutativity}
    \[
    A \cup B = B \cup A
    \]
    \[
    A \cap B = B \cap A
    \]

    \item \textbf{Associativity}
    \[
    (A \cup B) \cup C = A \cup (B \cup C)
    \]
    \[
    (A \cap B) \cap C = A \cap (B \cap C)
    \]

    \item \textbf{Distributivity}
    \[
    A \cup (B \cap C) = (A \cup B) \cap (A \cup C)
    \]
    \[
    A \cap (B \cup C) = (A \cap B) \cup (A \cap C)
    \]

    \item \textbf{Identity Laws}
    \[
    A \cap U = A
    \]
    \[
    A \cup \varnothing = A
    \]

    \item \textbf{Complement Laws}
    \[
    A \cup A^c = U
    \]
    \[
    A \cap A^c = \varnothing
    \]

    \item \textbf{Double Complement Law}
    \[
    (A^c)^c = A
    \]

    \item \textbf{Idempotence}
    \[
    A \cup A = A
    \]
    \[
    A \cap A = A
    \]

    \item \textbf{Universal Bound}
    \[
    A \cup U = U
    \]
    \[
    A \cap \varnothing = \varnothing
    \]

    \item \textbf{DeMorgan's Laws}
    \[
    (A \cup B)^c = A^c \cap B^c
    \]
    \[
    (A \cap B)^c = A^c \cup B^c
    \]

    \item \textbf{Absorption Laws}
    \[
    A \cup (A \cap B) = A
    \]
    \[
    A \cap (A \cup B) = A
    \]

    \item \textbf{Empty Set and Universal Set Negation}
    \[
    \varnothing^c = U
    \]
    \[
    U^c = \varnothing
    \]
 
\end{enumerate}


\end{document}